WIP

code/ecdsa/Hacl.Impl.EC.ScalarMultiplication.WNAF.fst
@@ -16,19 +16,30 @@ open Spec.ECC
 
 inline_for_extraction noextract
 let dradix_wnaf = (u64 64)
-inline_for_extraction noextract
-let dradix : (a: size_t)= (u32 32)
-noextract
-let lenPrecompWnaf = 16
+
 inline_for_extraction noextract
 let radix = (u64 5)
 
-open FStar.Mul
+inline_for_extraction noextract
+let dradix = size (pow2 (v radix))
 
+open FStar.Mul
 #set-options "--z3rlimit 100 --max_fuel 0 --max_ifuel 0" 
 
+noextract
+let lenPrecompWnaf: size_t = size (pow2 (v radix - 1))
 
-val uploadOne: #c: curve -> gen: point c -> b: lbuffer uint64 (getPointLenU64 c *. 16ul) -> Stack unit 
+
+let post_precomp_wnaf #c (b: Lib.Sequence.lseq uint64 (v (getPointLenU64 c) * v lenPrecompWnaf)) (generator : point_seq c) = 
+  let len = v (getPointLenU64 c) in
+  let generator = point_seq_as_nat c generator in 
+  forall (i: nat {i >= 0 && i < v lenPrecompWnaf}). 
+    let index = 2 * i + 1 in 
+    let pointZero = point_seq_as_nat c (Lib.Sequence.sub b (i * len) len) in 
+    pointEqual pointZero (point_mult #c index generator) 
+
+
+val uploadOne: #c: curve -> gen: point c -> b: lbuffer uint64 (getPointLenU64 c *. lenPrecompWnaf) -> Stack unit 
   (requires fun h -> live h gen /\ live h b /\ disjoint gen b /\ point_eval c h gen)
   (ensures fun h0 _ h1 -> modifies (loc b) h0 h1 /\ (
     let pointZero = gsub b (size 0) (getPointLenU64 c) in 
@@ -42,19 +53,13 @@ let uploadOne #c gen b =
   copy zeroP gen 
   
 
-let post_precomp_wnaf #c (b: Lib.Sequence.lseq uint64 (v (getPointLenU64 c) * lenPrecompWnaf)) (generator : point_seq c) = 
-  let len = v (getPointLenU64 c) in
-  let generator = point_seq_as_nat c generator in 
-  forall (i: nat {i >= 0 && i < lenPrecompWnaf}). 
-    let pointZero = point_seq_as_nat c (Lib.Sequence.sub b (i * len) len) in 
-    pointEqual pointZero (point_mult #c (i + 1) generator) 
+val generatePrecomputedTableRadix: #c: curve 
+  -> generator: point c
+  -> b: lbuffer uint64 (getPointLenU64 c *. lenPrecompWnaf) -> 
+  Stack unit  
+  (requires fun h -> live h generator /\ live h b /\ disjoint generator b)
+  (ensures fun h0 _ h1 -> modifies (loc b) h0 h1 /\ post_precomp_wnaf #c (as_seq h1 b) (as_seq h0 generator))
 
 
+let generatePrecomputedTableRadix #c generator b = admit()
 
-(*
-val precomp_wnaf: lbuffer uint64 ((getPointLenU64 P256 *. dradix) >>. 1ul) -> Stack unit 
-  (requires fun h -> True)
-  (ensures fun h0 _ h1 -> 
-
-
-let precomp_wnaf b = admit()
