code/ecdsa/Hacl.Impl.EC.ScalarMultiplication.Radix.fst
@@ -1,0 +1,41 @@
+module Hacl.Impl.EC.ScalarMultiplication.Radix
+
+open FStar.HyperStack.All
+open FStar.HyperStack
+module ST = FStar.HyperStack.ST
+
+open Lib.IntTypes
+open Lib.Buffer
+
+open Hacl.Spec.EC.Definition
+open Hacl.Impl.EC.MontgomeryLadder
+open Spec.ECC.Curves
+open Spec.ECC
+
+
+inline_for_extraction noextract
+let radix = 4ul
+
+let lenPrecompRadix = size (pow2 (v radix))
+
+open FStar.Mul
+#set-options "--z3rlimit 100 --max_fuel 0 --max_ifuel 0" 
+
+
+let post_precomp_radix #c (b: Lib.Sequence.lseq uint64 (v (getPointLenU64 c) * v lenPrecompRadix)) generator = 
+  let len = v (getPointLenU64 c) in
+  let generator = point_seq_as_nat c generator in 
+  forall (i: nat {i >= 0 && i < v lenPrecompRadix}). 
+    let pointZero = point_seq_as_nat c (Lib.Sequence.sub b (i * len) len) in 
+    pointEqual pointZero (point_mult #c i generator) 
+
+
+val generatePrecomputedTableRadix: #c: curve 
+  -> generator: point c
+  -> b: lbuffer uint64 (getPointLenU64 c *.lenPrecompRadix) -> 
+  Stack unit  
+  (requires fun h -> live h generator /\ live h b /\ disjoint generator b)
+  (ensures fun h0 _ h1 -> modifies (loc b) h0 h1 /\ post_precomp_radix #c (as_seq h1 b) (as_seq h0 generator))
+
+
+let generatePrecomputedTableRadix #c generator b = admit()
